Foundation/InterpretabilityLogic/Veltman/AxiomJ1.lean
@@ -9,27 +9,23 @@ variable {F : Veltman.Frame} {φ ψ χ : Formula ℕ}
 namespace Frame
 
 class HasAxiomJ1 (F : Frame) : Prop where
-  S_refl : ∀ x, IsRefl _ (F.S x)
-export HasAxiomJ1 (S_refl)
+  S_J1 : ∀ {x y}, x ≺ y → F.S x y y
+export HasAxiomJ1 (S_J1)
 
 end Frame
 
 @[simp high, grind]
 lemma validate_axiomJ1_of_J1 [F.HasAxiomJ1] : F ⊧ Axioms.J1 φ ψ := by
-  intro V x h y hy;
+  intro V x h₁ y Rxy h₂;
   use y;
   constructor;
-  . apply F.S_refl x |>.refl;
-  . apply h;
-    . exact y.2;
-    . exact hy;
+  . apply F.S_J1; assumption;
+  . apply h₁ <;> simpa;
 
 lemma Frame.HasAxiomJ1.of_validate_axiomJ1 (h : F ⊧ Axioms.J1 (.atom 0) (.atom 1)) : F.HasAxiomJ1 := by
   constructor;
-  intro x;
-  constructor;
-  intro y;
-  obtain ⟨z, Sxyz, hz⟩ := @h (λ u _ => u = y) x (by tauto) y (by tauto);
+  intro x y Rxy;
+  obtain ⟨z, Sxyz, hz⟩ := @h (λ u _ => u = y) x (by tauto) y Rxy (by tauto);
   replace hz : z = y := by
     simp only [Satisfies] at hz;
     grind;
