Foundation/InterpretabilityLogic/Veltman/AxiomJ4.lean
@@ -1,0 +1,72 @@
+import Foundation.InterpretabilityLogic.Veltman.Basic
+
+namespace LO.InterpretabilityLogic.Veltman
+
+open Veltman Formula.Veltman
+
+variable {F : Veltman.Frame} {φ ψ χ : Formula ℕ}
+
+namespace Frame
+
+class HasAxiomJ4 (F : Frame) : Prop where
+  S_J4 : ∀ {w x y}, (F.S w x y) → (w ≺ y)
+export HasAxiomJ4 (S_J4)
+
+end Frame
+
+@[simp high, grind]
+lemma validate_axiomJ4_of_HasAxiomJ4 [F.HasAxiomJ4] : F ⊧ Axioms.J4 φ ψ := by
+  intro V x h₁ h₂;
+  replace ⟨z, Rxz, h₂⟩ := Satisfies.dia_def.mp h₂;
+  obtain ⟨w, Sxzw, hw⟩ := h₁ z Rxz h₂;
+  apply Satisfies.dia_def.mpr;
+  use w;
+  constructor;
+  . apply F.S_J4 Sxzw;
+  . assumption;
+
+@[simp high, grind]
+lemma validate_axiomJ4Plus_of_HasAxiomJ4 [F.HasAxiomJ4] : F ⊧ Axioms.J4Plus φ ψ χ := by
+  intro V x h₁ h₂ y Rxy h₃;
+  obtain ⟨z, Sxyz, hz⟩ := h₂ y Rxy h₃;
+  use z;
+  constructor;
+  . assumption;
+  . apply h₁ z (F.S_J4 Sxyz) hz;
+
+@[simp high, grind]
+lemma Frame.HasAxiomJ4.of_validate_axiomJ4 (h : F ⊧ Axioms.J4 (.atom 0) (.atom 1)) : F.HasAxiomJ4 := by
+  constructor;
+  intro w x y Swxy;
+  have := @h (λ u a => match a with | 0 => u = x | 1 => u = y | _ => False) w ?_ ?_;
+  . obtain ⟨z, Rwz, hz⟩ := Satisfies.dia_def.mp this;
+    replace hz : z = y := by
+      simp [Semantics.Models, Satisfies] at hz;
+      grind;
+    apply hz ▸ Rwz;
+  . suffices ∀ (y_1 : F.World), w ≺ y_1 → y_1 = x → F.S w y_1 y by simpa [Satisfies];
+    rintro z Rwz rfl;
+    assumption;
+  . apply Satisfies.dia_def.mpr;
+    use x;
+    constructor;
+    . apply F.S_cond Swxy;
+    . tauto;
+
+open Formula (atom)
+lemma validate_axiomJ4_of_validate_axiomJ4Plus {F : Veltman.Frame} (h : F ⊧ Axioms.J4Plus (.atom 1) (.atom 2) (.atom 0)) : F ⊧ Axioms.J4 (.atom 0) (.atom 1) := by
+
+  intro V x h₁ h₂;
+  dsimp [Axioms.J4Plus] at h;
+
+  have := h V x (by sorry);
+  replace ⟨z, Rxz, h₂⟩ := Satisfies.dia_def.mp h₂;
+  obtain ⟨w, Sxzw, hw⟩ := h₁ z Rxz h₂;
+  apply Satisfies.dia_def.mpr;
+  use w;
+  constructor;
+  . apply F.trans Rxz;
+    sorry;
+  . assumption;
+
+end LO.InterpretabilityLogic.Veltman
