Foundation/InterpretabilityLogic/Veltman/Logic/ILMinus_J4Plus.lean
@@ -1,5 +1,6 @@
 import Foundation.InterpretabilityLogic.Veltman.Logic.ILMinus
-import Foundation.InterpretabilityLogic.Veltman.AxiomJ1
+import Foundation.InterpretabilityLogic.Veltman.AxiomJ4
+
 
 namespace LO.InterpretabilityLogic
 
@@ -8,44 +9,44 @@ open Veltman
 
 namespace Veltman
 
-protected abbrev FrameClass.ILMinus_J1 : FrameClass := { F | F.HasAxiomJ1 }
+protected abbrev FrameClass.ILMinus_J4Plus : FrameClass := { F | F.HasAxiomJ4 }
 
-instance : trivialFrame.HasAxiomJ1 where
-  S_J1 := by tauto
+instance : trivialFrame.HasAxiomJ4 where
+  S_J4 {w x y} Swxy := by have := x.2; contradiction;
 
 end Veltman
 
 
 open Hilbert.Minimal
 
-namespace ILMinus_J1
+namespace ILMinus_J4Plus
 
-instance Veltman.sound : Sound InterpretabilityLogic.ILMinus_J1 FrameClass.ILMinus_J1 := by
+instance Veltman.sound : Sound InterpretabilityLogic.ILMinus_J4Plus FrameClass.ILMinus_J4Plus := by
   apply Veltman.instFrameClassSound;
   constructor;
   intro φ hφ F hF;
   replace hF := Set.mem_setOf_eq.mp hF;
   rcases (by simpa [buildAxioms] using hφ) with (rfl | rfl | rfl | rfl) <;> simp;
 
-instance : Entailment.Consistent InterpretabilityLogic.ILMinus_J1 := Veltman.consistent_of_sound_frameclass FrameClass.ILMinus_J1 $ by
+instance : Entailment.Consistent InterpretabilityLogic.ILMinus_J4Plus := Veltman.consistent_of_sound_frameclass FrameClass.ILMinus_J4Plus $ by
   use Veltman.trivialFrame;
   apply Set.mem_setOf_eq.mpr;
   infer_instance;
 
-end ILMinus_J1
+end ILMinus_J4Plus
 
-instance : InterpretabilityLogic.ILMinus ⪱ InterpretabilityLogic.ILMinus_J1 := by
+instance : InterpretabilityLogic.ILMinus ⪱ InterpretabilityLogic.ILMinus_J4Plus := by
   constructor;
   . apply weakerThan_of_subset_axioms $ by grind;
   . apply Entailment.not_weakerThan_iff.mpr;
-    use (Axioms.J1 (.atom 0) (.atom 1));
+    use (Axioms.J4Plus (.atom 0) (.atom 1) (.atom 2));
     constructor;
     . simp;
     . apply Sound.not_provable_of_countermodel (𝓜 := Veltman.FrameClass.ILMinus);
       apply Veltman.not_validOnFrameClass_of_exists_frame;
       use {
         toKripkeFrame := {
-          World := Fin 2
+          World := Fin 3
           Rel := λ x y => x < y
         }
         isGL := Modal.Kripke.Frame.isGL_of_isFiniteGL {
@@ -53,12 +54,11 @@ instance : InterpretabilityLogic.ILMinus ⪱ InterpretabilityLogic.ILMinus_J1 :=
           irrefl := by omega;
         }
         S _ _ _ := False
-        S_cond := by tauto
       }
       constructor;
       . tauto;
       . by_contra hC;
-        replace hC := Veltman.Frame.HasAxiomJ1.of_validate_axiomJ1 hC |>.S_J1 (show 0 < 1 by omega);
-        simp at hC;
+        replace hC : ¬1 < 2 := Veltman.Frame.HasAxiomJ4.of_validate_axiomJ4 hC |>.S_J4Plus 0 ⟨1, by omega⟩ ⟨2, by omega⟩;
+        omega;
 
 end LO.InterpretabilityLogic
